state is becoming global again

ObcToClight/Generation.v
@@ -312,7 +312,7 @@ Definition load_in (ins: list (ident * type)): Clight.statement :=
 
 Definition write_out (node: ident) (outs: list (ident * type))
   : Clight.statement :=
-  let out_struct := Ident.prefix out step in
+  let out_struct := glob_id (Ident.prefix out step) in
   let t_struct := type_of_inst (prefix_fun node step) in
   fold_right
     (fun (xt: ident * type) s =>
@@ -327,12 +327,12 @@ Definition write_out (node: ident) (outs: list (ident * type))
     ) Clight.Sskip outs.
 
 Definition reset_call (node: ident): Clight.statement :=
-  let p_self := Clight.Eaddrof (Clight.Evar self (type_of_inst node)) (type_of_inst_p node) in
+  let p_self := Clight.Eaddrof (Clight.Evar (glob_id self) (type_of_inst node)) (type_of_inst_p node) in
   funcall None (prefix_fun node reset) [p_self].
 
 Definition step_call (node: ident) (args: list Clight.expr) (m_out: list (ident * type)): Clight.statement :=
-  let p_self := Clight.Eaddrof (Clight.Evar self (type_of_inst node)) (type_of_inst_p node) in
-  let out_struct := Ident.prefix out step in
+  let p_self := Clight.Eaddrof (Clight.Evar (glob_id self) (type_of_inst node)) (type_of_inst_p node) in
+  let out_struct := glob_id (Ident.prefix out step) in
   let t_struct := type_of_inst (prefix_fun node step) in
   let p_out := Clight.Eaddrof (Clight.Evar out_struct t_struct) (pointer_of t_struct) in
   match m_out with
@@ -363,7 +363,7 @@ Definition make_main (node: ident) (m: method): AST.globdef Clight.fundef Ctypes
                      (Ident.prefix out step, type_of_inst (prefix_fun node step)) :: []
                    end
   in
-  fundef [] vars (map translate_param m.(m_in)) Ctypes.type_int32s body.
+  fundef [] [] (map translate_param m.(m_in)) Ctypes.type_int32s body.
 
 Definition vardef (env: Ctypes.composite_env) (volatile: bool) (x: ident * Ctypes.type)
   : ident * AST.globdef Clight.fundef Ctypes.type :=
@@ -399,19 +399,21 @@ Fixpoint check_size_env (env: Ctypes.composite_env) (types: list Ctypes.composit
 
 Definition make_program'
            (types: list Ctypes.composite_definition)
-           (gvars_vol: list (ident * Ctypes.type))
+           (gvars gvars_vol: list (ident * Ctypes.type))
            (defs: list (ident * AST.globdef Clight.fundef Ctypes.type))
            (public: idents)
            (main: ident) : res (Ctypes.program Clight.function) :=
   match build_composite_env' types with
   | inl (exist ce P) => 
     do _ <- check_size_env ce types;
-    OK {| Ctypes.prog_defs := map (vardef ce true) gvars_vol ++ defs;
-                 Ctypes.prog_public := public;
-                 Ctypes.prog_main := main;
-                 Ctypes.prog_types := types;
-                 Ctypes.prog_comp_env := ce;
-                 Ctypes.prog_comp_env_eq := P |}
+      OK {| Ctypes.prog_defs := map (vardef ce false) gvars ++
+                                map (vardef ce true) gvars_vol ++
+                                defs;
+            Ctypes.prog_public := public;
+            Ctypes.prog_main := main;
+            Ctypes.prog_types := types;
+            Ctypes.prog_comp_env := ce;
+            Ctypes.prog_comp_env_eq := P |}
   | inr msg => Error msg
   end.
 
@@ -422,13 +424,23 @@ Definition translate (main_node: ident) (prog: program): res Clight.program :=
     | Some m =>
       match find_method reset c.(c_methods) with
       | Some _ =>
+        let f := glob_id self in
+        let step_out := glob_id (Ident.prefix out step) in
+        let f_gvar := (f, type_of_inst main_node) in
+        let step_out_gvar := (step_out, type_of_inst (prefix_fun main_node step)) in
         let ins := map glob_bind m.(m_in) in
         let outs := map glob_bind m.(m_out) in
         let main := make_main main_node m in
         let cs := map (translate_class prog) prog in
         let (structs, funs) := split cs in
         let gdefs := concat funs ++ [(main_id, main)] in
-        make_program' (concat structs) (outs ++ ins) gdefs [] main_id
+        make_program' (concat structs)
+                      (f_gvar
+                         :: match m.(m_out) with
+                            | [] => []
+                            | _ => [step_out_gvar]
+                            end)
+                      (outs ++ ins) gdefs [] main_id
       | None => Error (msg "ObcToClight: reset function not found")
       end
     | None => Error (msg "ObcToClight: step function not found")
