ObcToClight/Correctness.v
@@ -396,8 +396,8 @@ Section PRESERVATION.
   Hypothesis WT: wt_program prog.
   
   Lemma build_check_size_env_ok:
-    forall types gvars_vol defs public main p,
-      make_program' types gvars_vol defs public main = Errors.OK p ->
+    forall types gvars gvars_vol defs public main p,
+      make_program' types gvars gvars_vol defs public main = Errors.OK p ->
       build_composite_env types = Errors.OK p.(prog_comp_env)
       /\ check_size_env p.(prog_comp_env) types = Errors.OK tt.
   Proof.
@@ -408,21 +408,21 @@ Section PRESERVATION.
   Qed.
 
   Lemma build_ok:
-    forall types gvars_vol defs public main p,
-      make_program' types gvars_vol defs public main = Errors.OK p ->
+    forall types gvars gvars_vol defs public main p,
+      make_program' types gvars gvars_vol defs public main = Errors.OK p ->
       build_composite_env types = Errors.OK p.(prog_comp_env).
   Proof.
     intros ** H.
-    apply (proj1 (build_check_size_env_ok _ _ _ _ _ _ H)).
+    apply (proj1 (build_check_size_env_ok _ _ _ _ _ _ _ H)).
   Qed.
 
   Lemma check_size_env_ok:
-    forall types gvars_vol defs public main p,
-      make_program' types gvars_vol defs public main = Errors.OK p ->
+    forall types gvars gvars_vol defs public main p,
+      make_program' types gvars gvars_vol defs public main = Errors.OK p ->
       check_size_env p.(prog_comp_env) types = Errors.OK tt.
   Proof.
     intros ** H.
-    apply (proj2 (build_check_size_env_ok _ _ _ _ _ _ H)).
+    apply (proj2 (build_check_size_env_ok _ _ _ _ _ _ _ H)).
   Qed.
 
   Lemma check_size_ok:
@@ -549,6 +549,13 @@ Section PRESERVATION.
       + apply M.add_1; auto.
   Qed.
 
+  Hypothesis main_methods_glob_not_prefixed:
+    forall c cls,
+      find_class main_node prog = Some (c, cls) ->
+      forall f m,
+        find_method f (c_methods c) = Some m ->
+        Forall (fun xt => ~ prefixed (fst xt)) (m.(m_in) ++ m.(m_out)).
+  
   Lemma prog_defs_norepet:
     list_norepet (map fst (prog_defs tprog)).
   Proof.
@@ -561,31 +568,85 @@ Section PRESERVATION.
     inversion_clear TRANSL; simpl.
     rewrite 4 map_app, <-app_assoc, <-NoDup_norepet.
     repeat rewrite glob_bind_vardef_fst; simpl.
-    repeat apply NoDup_app'; repeat apply Forall_not_In_app;
-      repeat apply Forall_not_In_singleton.
-    - apply NoDup_glob_id, m_nodupout.
-    - apply NoDup_glob_id, m_nodupin.
-    - rewrite Funs.
-      now apply NoDup_funs.
-    - repeat constructor; auto.
-    - intro Hin; subst funs; apply prefixed_funs in Hin.
-      inversion Hin as [? ? E].
-      unfold prefix, main_id in E.
-      unfold prefix_fun, fun_id in E.
-      apply pos_of_str_injective in E; rewrite pos_to_str_equiv in E.
-      inversion E.
-    - apply glob_not_in_prefixed, all_In_Forall; intros ** Hin.
-      apply prefixed_fun_prefixed; subst funs.
-      now apply prefixed_funs in Hin.
-    - apply main_not_glob. 
-    - apply NoDupMembers_glob.
-      pose proof (m_nodupvars m) as Nodup.
-      rewrite NoDupMembers_app_assoc, <-app_assoc in Nodup.
-      now apply NoDupMembers_app_r, NoDupMembers_app_assoc in Nodup.
-    - apply glob_not_in_prefixed, all_In_Forall; intros ** Hin.
-      apply prefixed_fun_prefixed; subst funs.
-      now apply prefixed_funs in Hin.
-    - apply main_not_glob.
+    specialize (main_methods_glob_not_prefixed c cls eq_refl).
+    apply main_methods_glob_not_prefixed in Estep.
+    assert ( ~ In (glob_id self)
+               (map (fun xt => glob_id (fst xt)) (m_out m) ++
+                map (fun xt => glob_id (fst xt)) (m_in m) ++
+                map fst (concat funs) ++
+                [main_id])) as Notin_self.
+    { pose proof (m_notreserved self m (in_eq self _)) as Res; unfold meth_vars in Res.
+      repeat rewrite in_app_iff, in_map_iff; rewrite In_singleton;
+        intros [((x, t) & E & Hin)|[((x, t) & E & Hin)|[((x, t) & E & Hin)|Hin]]];
+        try simpl in E.
+      - apply glob_id_injective in E; subst x.
+        apply In_InMembers in Hin.
+        apply Res; now repeat (rewrite InMembers_app; right).
+      - apply glob_id_injective in E; subst x.
+        apply In_InMembers in Hin.
+        apply Res; now rewrite InMembers_app; left.
+      - subst x.
+        apply in_map with (f:=fst) in Hin.
+        subst funs. apply prefixed_funs, prefixed_fun_prefixed in Hin.
+        contradict Hin; apply glob_id_not_prefixed. 
+      - unfold glob_id, main_id in Hin.
+        apply pos_of_str_injective in Hin.
+        inv Hin.
+    }
+    assert (NoDup (map (fun xt => glob_id (fst xt)) (m_out m) ++
+                   map (fun xt => glob_id (fst xt)) (m_in m) ++
+                   map fst (concat funs) ++
+                   [main_id])) as Nodup.
+    { repeat apply NoDup_app'; repeat apply Forall_not_In_app;
+        repeat apply Forall_not_In_singleton.
+      - apply NoDup_glob_id, m_nodupout.
+      - apply NoDup_glob_id, m_nodupin.
+      - rewrite Funs.
+        now apply NoDup_funs.
+      - repeat constructor; auto.
+      - intro Hin; subst funs; apply prefixed_funs in Hin.
+        inversion Hin as [? ? E].
+        unfold prefix, main_id in E.
+        unfold prefix_fun, fun_id in E.
+        apply pos_of_str_injective in E; rewrite pos_to_str_equiv in E.
+        inversion E.
+      - apply glob_not_in_prefixed, all_In_Forall; intros ** Hin.
+        apply prefixed_fun_prefixed; subst funs.
+        now apply prefixed_funs in Hin.
+      - apply main_not_glob. 
+      - apply NoDupMembers_glob.
+        pose proof (m_nodupvars m) as Nodup.
+        rewrite NoDupMembers_app_assoc, <-app_assoc in Nodup.
+        now apply NoDupMembers_app_r, NoDupMembers_app_assoc in Nodup.
+      - apply glob_not_in_prefixed, all_In_Forall; intros ** Hin.
+        apply prefixed_fun_prefixed; subst funs.
+        now apply prefixed_funs in Hin.
+      - apply main_not_glob.
+    }
+    case_eq (m_out m); intros ** Out; rewrite map_app.
+    - simpl; repeat constructor; rewrite Out in Notin_self, Nodup; auto.
+    - rewrite <-Out; simpl. repeat constructor; auto.
+      + repeat rewrite not_in_cons; repeat split; auto.
+        intro E; apply glob_id_injective in E.
+        apply self_not_prefixed; rewrite E; constructor.
+      + repeat rewrite in_app_iff, in_map_iff; rewrite In_singleton;
+          intros [((x, t) & E & Hin)|[((x, t) & E & Hin)|[((x, t) & E & Hin)|Hin]]];
+          try simpl in E.
+        * apply glob_id_injective in E; subst x.
+          apply (In_Forall (prefix out step, t)) in Estep.
+          2: rewrite in_app; now right.
+          apply Estep; simpl; constructor.
+        * apply glob_id_injective in E; subst x.
+          apply (In_Forall (prefix out step, t)) in Estep.
+          2: rewrite in_app; now left.
+          apply Estep; simpl; constructor.
+        * subst x.
+          apply in_map with (f:=fst) in Hin.
+          subst funs; apply prefixed_funs, prefixed_fun_prefixed in Hin.
+          contradict Hin; apply glob_id_not_prefixed.
+        * unfold glob_id, main_id in Hin.
+          apply pos_of_str_injective in Hin.
+          inv Hin.
   Qed.
   Hint Resolve prog_defs_norepet.
   
@@ -773,7 +834,7 @@ Section PRESERVATION.
           unfold AST.prog_defmap; simpl.
           apply PTree_Properties.of_list_norepet; auto.
           inversion_clear TRANSL.
-          apply in_app; right; apply in_app; left.
+          apply in_cons, in_app; right; apply in_app; right; apply in_app; left.
           unfold translate_method in Findmth; auto.
         }
         apply Genv.find_def_symbol in Hget.
@@ -3534,11 +3595,11 @@ Section PRESERVATION.
   Qed.
 
   Lemma make_program_defs:
-    forall types gvars_vol defs public main p,
-      make_program' types gvars_vol defs public main = Errors.OK p ->
+    forall types gvars gvars_vol defs public main p,
+      make_program' types gvars gvars_vol defs public main = Errors.OK p ->
       exists gce,
         build_composite_env types = Errors.OK gce
-        /\ p.(AST.prog_defs) = map (vardef gce true) gvars_vol ++ defs.
+        /\ p.(AST.prog_defs) = map (vardef gce false) gvars ++ map (vardef gce true) gvars_vol ++ defs.
   Proof.
     unfold make_program'; intros.
     destruct (build_composite_env' types) as [[gce ?]|?]; try discriminate.
@@ -3820,12 +3881,7 @@ Section PRESERVATION.
               /\ main.(fn_return) = type_int32s
               /\ main.(fn_callconv) = AST.cc_default
               /\ main.(fn_params) = []
-              /\ main.(fn_vars) = (self, type_of_inst main_node)
-                                   :: match m_out m_step with
-                                      | [] => []
-                                      | _ => [(prefix out step,
-                                             type_of_inst (prefix_fun main_node step))]
-                                      end
+              /\ main.(fn_vars) = []
               /\ main.(fn_temps) = map translate_param (m_in m_step)
               /\ main.(fn_body) =
                  return_zero
@@ -3873,7 +3929,7 @@ Section PRESERVATION.
         apply PTree_Properties.of_list_norepet; auto.
         inversion_clear TRANSL; auto; simpl.
         rewrite map_app.
-        apply in_app; left; apply in_app; right.
+        apply in_cons, in_app; right; apply in_app; left; apply in_app; right.
         apply in_map_iff.
         exists (glob_id x, cltype t); split; auto.
         apply in_map_iff.
@@ -3902,7 +3958,7 @@ Section PRESERVATION.
         apply PTree_Properties.of_list_norepet; auto.
         inversion_clear TRANSL; auto; simpl.
         rewrite map_app.
-        apply in_app; left; apply in_app; left.
+        apply in_cons, in_app; right; apply in_app; left; apply in_app; left.
         apply in_map_iff.
         exists (glob_id x, cltype t); split; auto.
         apply in_map_iff.
@@ -3924,7 +3980,7 @@ Section PRESERVATION.
       { unfold AST.prog_defmap; simpl; split;
           [apply PTree_Properties.of_list_norepet; auto|];
           inversion_clear TRANSL; auto.
-        apply in_app; right; apply in_app; right; apply in_eq.
+        apply in_cons, in_app; right; apply in_app; right; apply in_app; right; apply in_eq.
       }
       rewrite Hmain_id.
       apply Genv.find_def_symbol in Hget.
